TypeInferencer.v
@@ -12,14 +12,14 @@ Require Import AST.
 Require Import Maps.
 
 
-Inductive typeinf : environment -> nat -> ut_expr -> (nat * type * constraint) % type -> Prop :=
+Inductive typeinf : ti_env -> nat -> ut_expr -> (nat * inft_type * constr) % type -> Prop :=
   (* ut_Num *)
   (* ut_Bool *)
   (* ut_Var *)
   | TI_Num: forall env n fv,
-    typeinf env fv  (ut_Num n) (fv, TNum, [])
+    typeinf env fv (ut_Num n) (fv, inft_Num, [])
   | TI_Bool: forall env b fv,
-    typeinf env fv  (ut_Bool b) (fv, TBool, [])
+    typeinf env fv (ut_Bool b) (fv, inft_Bool, [])
   | TI_Var: forall env x fv T,
     env x = Some T -> typeinf env fv (ut_Var x) (fv, T, [])
 
@@ -32,14 +32,14 @@ Inductive typeinf : environment -> nat -> ut_expr -> (nat * type * constraint) %
     typeinf env fv c (c_fv, c_T, c_C) ->
     typeinf env c_fv  e1 (e1_fv, e1_T, e1_C) ->
     typeinf env e1_fv  e2 (e2_fv, e2_T, e2_C) ->
-    typeinf env fv (ut_If c e1 e2) (e2_fv, e1_T, e2_C ++ e1_C ++ c_C ++ [(e1_T, e2_T); (c_T, TBool)])
+    typeinf env fv (ut_If c e1 e2) (e2_fv, e1_T, e2_C ++ e1_C ++ c_C ++ [(e1_T, e2_T); (c_T, inft_Bool)])
 
   (* ut_Fun *)
   | TI_Fun:
     forall env fv
       x e e_fv e_C e_T,
-    typeinf (update env x (TVar (Id fv))) (fv + 1)  e (e_fv, e_T, e_C) ->
-    typeinf env fv (ut_Fun x e) (e_fv, (TFun (TVar (Id fv)) e_T), e_C)
+    typeinf (update env x (inft_Var (Id fv))) (fv + 1)  e (e_fv, e_T, e_C) ->
+    typeinf env fv (ut_Fun x e) (e_fv, (inft_Fun (inft_Var (Id fv)) e_T), e_C)
 
   (* ut_Call *)
   | TI_Call:
@@ -48,7 +48,7 @@ Inductive typeinf : environment -> nat -> ut_expr -> (nat * type * constraint) %
       e e_fv e_C e_T,
     typeinf env fv f (f_fv, f_T, f_C) ->
     typeinf env f_fv e (e_fv, e_T, e_C) ->
-    typeinf env fv (ut_Call f e) (e_fv + 1, TVar (Id e_fv), e_C ++ f_C ++ [(f_T, TFun e_T (TVar (Id e_fv)))])
+    typeinf env fv (ut_Call f e) (e_fv + 1, inft_Var (Id e_fv), e_C ++ f_C ++ [(f_T, inft_Fun e_T (inft_Var (Id e_fv)))])
 
   (* ut_Cons *)
   | TI_Cons:
@@ -57,12 +57,12 @@ Inductive typeinf : environment -> nat -> ut_expr -> (nat * type * constraint) %
       tl tl_fv tl_C tl_T,
     typeinf env fv hd (hd_fv, hd_T, hd_C) ->
     typeinf env hd_fv tl (tl_fv, tl_T, tl_C) ->
-    typeinf env fv (ut_Cons hd tl) (tl_fv, TList hd_T, tl_C ++ hd_C ++ [(tl_T, TList hd_T)])
+    typeinf env fv (ut_Cons hd tl) (tl_fv, inft_List hd_T, tl_C ++ hd_C ++ [(tl_T, inft_List hd_T)])
 
   (* ut_Nil *)
   | TI_Nil:
     forall env fv,
-    typeinf env fv ut_Nil (fv + 1, TList (TVar (Id fv)), [])
+    typeinf env fv ut_Nil (fv + 1, inft_List (inft_Var (Id fv)), [])
 
   (* ut_Binop *)
   | TI_Binop_nnn:
@@ -70,25 +70,20 @@ Inductive typeinf : environment -> nat -> ut_expr -> (nat * type * constraint) %
       e1 e1_fv e1_C e1_T
       e2 e2_fv e2_C e2_T,
     op = op_Plus \/
-    op = op_Minus \/
-    op = op_Mult \/
-    op = op_Div \/
-    op = op_Mod ->
+    op = op_Minus ->
     typeinf env fv e1 (e1_fv, e1_T, e1_C) ->
     typeinf env e1_fv e2 (e2_fv, e2_T, e2_C) ->
-    typeinf env fv (ut_Binop op e1 e2) (e2_fv, TNum, e2_C++ e1_C ++ [(e2_T, TNum); (e1_T, TNum)])
+    typeinf env fv (ut_Binop op e1 e2) (e2_fv, inft_Num, e2_C++ e1_C ++ [(e2_T, inft_Num); (e1_T, inft_Num)])
 
   | TI_Binop_nnb:
     forall env fv op
       e1 e1_fv e1_C e1_T
       e2 e2_fv e2_C e2_T,
     op = op_Eq \/
-    op = op_Neq \/
-    op = op_Lt \/
-    op = op_Gt ->
+    op = op_Neq ->
     typeinf env fv e1 (e1_fv, e1_T, e1_C) ->
     typeinf env e1_fv e2 (e2_fv, e2_T, e2_C) ->
-    typeinf env fv (ut_Binop op e1 e2) (e2_fv, TBool, e2_C++ e1_C ++ [(e2_T, TNum); (e1_T, TNum)])
+    typeinf env fv (ut_Binop op e1 e2) (e2_fv, inft_Bool, e2_C++ e1_C ++ [(e2_T, inft_Num); (e1_T, inft_Num)])
 
   | TI_Binop_bbb:
     forall env fv op
@@ -98,87 +93,23 @@ Inductive typeinf : environment -> nat -> ut_expr -> (nat * type * constraint) %
     op = op_Or ->
     typeinf env fv e1 (e1_fv, e1_T, e1_C) ->
     typeinf env e1_fv e2 (e2_fv, e2_T, e2_C) ->
-    typeinf env fv (ut_Binop op e1 e2) (e2_fv, TBool, e2_C++ e1_C ++ [(e2_T, TBool); (e1_T, TBool)]).
+    typeinf env fv (ut_Binop op e1 e2) (e2_fv, inft_Bool, e2_C++ e1_C ++ [(e2_T, inft_Bool); (e1_T, inft_Bool)]).
 
-Fixpoint occurs (i : id) (t : type) : bool :=
+Fixpoint subst (s : (id * inft_type) % type) (t : inft_type) : inft_type :=
   match t with
-    | TNum | TBool => false
-    | TFun x e => orb (occurs i x) (occurs i e)
-    | TList l => occurs i l
-    | TVar x => beq_id i x
+    | inft_Num | inft_Bool => t
+    | inft_Fun x e => inft_Fun (subst s x) (subst s e)
+    | inft_List l => inft_List (subst s l)
+    | inft_Var x => let (i, sub) := s in if beq_id i x then sub else t
   end.
 
-Fixpoint subst (s : (id * type) % type) (t : type) : type :=
-  let (i, sub) := s in
-    match t with
-      | TNum | TBool => t
-      | TFun x e => TFun (subst s x) (subst s e)
-      | TList l => TList (subst s l)
-      | TVar x => if beq_id i x then sub else t
-    end.
-
-Definition app_substs (sub : substitution) (tp : type) : type :=
+Definition app_substs (sub : substs) (tp : inft_type) : inft_type :=
   fold_right (fun s t => subst s t) tp sub.
 
-Inductive solution : substitution -> constraint -> Prop :=
+Inductive solution : substs -> constr -> Prop :=
   | SOL_Empty: forall s, solution s []
   | SOL_NotEmpty:
     forall s t1 t2 tl,
     app_substs s t1 = app_substs s t2 ->
     solution s tl ->
     solution s ((t1, t2)::tl).
-
-(* Process constraints from right to left *)
-Inductive unify : constraint -> substitution -> Prop :=
-  | U_Empty: unify [] []
-
-  (* (TNum, TNum) *)
-  (* (TBool, TBool) *)
-  (* (S, S) *)
-  (* (TVar i, TVar i) *)
-  | U_Identical:
-    forall t1 t2 t tl tl_sub,
-    unify tl tl_sub ->
-    app_substs tl_sub t1 = t ->
-    app_substs tl_sub t2 = t ->
-    unify ((t1, t2)::tl) tl_sub
-
-  (* (TFun x1 e1, TFun x2 e2) *)
-  | U_FunFun:
-    forall t1 t2 tl tl_sub
-      x1 e1 x2 e2 fun_sub,
-    unify tl tl_sub ->
-    app_substs tl_sub t1 = TFun x1 e1 ->
-    app_substs tl_sub t2 = TFun x2 e2 ->
-    unify [(x1, x2);(e1, e2)] fun_sub ->
-    unify ((t1, t2)::tl) (fun_sub ++ tl_sub)
-
-  (* (TList l1, TList l2) *)
-  | U_ListList:
-    forall t1 t2 tl tl_sub
-      l1 l2 list_sub,
-    unify tl tl_sub ->
-    app_substs tl_sub t1 = TList l1 ->
-    app_substs tl_sub t2 = TList l2 ->
-    unify [(l1, l2)] list_sub ->
-    unify ((t1, t2)::tl) (list_sub ++ tl_sub)
-
-  (* (TVar x, _) *)
-  | U_VarLeft:
-    forall t1 t2 tl tl_sub
-      x T,
-    unify tl tl_sub ->
-    app_substs tl_sub t1 = TVar x ->
-    app_substs tl_sub t2 = T ->
-    occurs x T = false ->
-    unify ((t1, t2)::tl) ((x, T)::tl_sub)
-
-  (* (_, TVar x) *)
-  | U_VarRight:
-    forall t1 t2 tl tl_sub
-      x T,
-    unify tl tl_sub ->
-    app_substs tl_sub t1 = T ->
-    app_substs tl_sub t2 = TVar x ->
-    occurs x T = false ->
-    unify ((t1, t2)::tl) ((x, T)::tl_sub).
