Proofs.v
@@ -18,61 +18,18 @@ Require Import TypeChecker.
 (* ################################################################# *)
 (* Small proofs *)
 
-(* occurs *)
-Lemma occurs_nontvar : forall i t, vartype t = false -> occurs i t = false.
-Proof.
-  introv H.
-  induction t.
-  - reflexivity.
-  - reflexivity.
-  - simpl. apply orb_false_iff. split.
-    * inversion H. apply orb_false_iff in H1. destruct H1.
-      rewrite H0. rewrite H1. simpl. apply IHt1. assumption.
-    * inversion H. apply orb_false_iff in H1. destruct H1.
-      rewrite H0. rewrite H1. simpl. apply IHt2. assumption.
-  - simpl. inversion H. rewrite H1. apply IHt. assumption.
-  - inversion H.
-Qed.
-
-(* subst *)
-Lemma subst_vartype_false : forall i t t', vartype t = false  -> subst (i, t') t = t.
-Proof.
-  introv Hvt.
-  induction t.
-  - reflexivity.
-  - reflexivity.
-  - inversion Hvt. apply orb_false_iff in H0. destruct H0.
-    intuition. simpl. rewrite H1, H2. reflexivity.
-  - inversion Hvt. intuition. simpl. rewrite H. reflexivity.
-  - inversion Hvt.
-Qed.
-
 (* app_substs *)
-Lemma app_substs_nontvar : forall s t, vartype t = false -> app_substs s t = t.
-Proof.
-  introv H.
-  induction s as [|hd tl].
-  - reflexivity.
-  - destruct t.
-    * simpl. rewrite IHtl. destruct hd. apply subst_vartype_false. assumption.
-    * simpl. rewrite IHtl. destruct hd. apply subst_vartype_false. assumption.
-    * simpl. rewrite IHtl. destruct hd. apply subst_vartype_false. assumption.
-    * simpl. rewrite IHtl. destruct hd. apply subst_vartype_false. assumption.
-    * inversion H.
-Qed.
-
-(* app_substs *)
-Example app_substs_ex1 : app_substs [(Id 1, TNum)] (TFun (TVar (Id 1)) TNum) = TFun TNum TNum.
+Example app_substs_ex1 : app_substs [(Id 1, inft_Num)] (inft_Fun (inft_Var (Id 1)) inft_Num) = inft_Fun inft_Num inft_Num.
 Proof. reflexivity. Qed.
 
-Example app_substs_ex2 : app_substs [(Id 1, TNum);(Id 2, TBool)] (TFun (TVar (Id 1)) (TVar (Id 2))) = TFun TNum TBool.
+Example app_substs_ex2 : app_substs [(Id 1, inft_Num);(Id 2, inft_Bool)] (inft_Fun (inft_Var (Id 1)) (inft_Var (Id 2))) = inft_Fun inft_Num inft_Bool.
 Proof. reflexivity. Qed.
 
 (* solution *)
 Example solution_ex1 :
   solution
-    [(Id 1, TNum); (Id 2, TNum); (Id 3, TNum)]
-    [(TList (TVar (Id 1)), TList TNum); (TList (TVar (Id 3)), TList TNum); (TVar (Id 2), TNum)].
+    [(Id 1, inft_Num); (Id 2, inft_Num); (Id 3, inft_Num)]
+    [(inft_List (inft_Var (Id 1)), inft_List inft_Num); (inft_List (inft_Var (Id 3)), inft_List inft_Num); (inft_Var (Id 2), inft_Num)].
 Proof.
   apply SOL_NotEmpty.
   - reflexivity.
@@ -83,133 +40,198 @@ Proof.
       + apply SOL_Empty.
 Qed.
 
+(* convert_type *)
+Lemma exists_inf_type_to_cont_type :
+  forall ct, exists it, convert_type it ct.
+Proof.
+  introv.
+  induction ct.
+  - exists inft_Num. apply CT_Num.
+  - exists inft_Bool. apply CT_Bool.
+  - destruct IHct1. destruct IHct2. exists (inft_Fun x x0). apply CT_Fun.
+    * assumption.
+    * assumption.
+  - destruct IHct. exists (inft_List x). apply CT_List. assumption.
+Qed.
+
+(* convert_expr *)
+Lemma exists_type_for_nil :
+  forall t, convert_expr t ut_Nil -> exists t', t = t_Nil t'.
+Proof.
+  introv H. inverts H. exists t0. reflexivity.
+Qed.
+
+(* substs *)
+Lemma subst_nontvar : 
+  forall x y TI, (exists TC, convert_type TI TC) -> subst (x, y) TI = TI.
+Proof.
+  introv Hvt.
+  induction TI.
+  - reflexivity.
+  - reflexivity.
+  - inverts Hvt. inverts H. simpl.
+    assert (Htc1: exists tc, convert_type TI1 tc). { exists x_t. assumption. }
+    assert (Htc2: exists tc, convert_type TI2 tc). { exists e_t. assumption. }
+    apply IHTI1 in Htc1.
+    apply IHTI2 in Htc2.
+    rewrite Htc1, Htc2.
+    reflexivity.
+  - inverts Hvt. inverts H. simpl.
+    assert (Htc: exists tc, convert_type TI tc). { exists l_t. assumption. }
+    apply IHTI in Htc.
+    rewrite Htc.
+    reflexivity.
+  - inverts Hvt. inverts H.
+Qed.
+
+Lemma subst_form_list :
+  forall x y t, exists t', subst (x, y) (inft_List t) = inft_List t'.
+Proof.
+  introv.
+  induction t.
+  - exists inft_Num. reflexivity.
+  - exists inft_Bool. reflexivity.
+  - destruct IHt1. destruct IHt2.
+    exists (inft_Fun x0 x1).
+    simpl. simpl in H. simpl in H0.
+    inverts H. inverts H0.
+    reflexivity.
+  - destruct IHt.
+    exists (inft_List x0).
+    simpl. simpl in H.
+    rewrite H. reflexivity.
+  - simpl. induction beq_id.
+    * exists y. reflexivity.
+    * exists (inft_Var i). reflexivity.
+Qed.
+
+
+(* app_substs *)
+Lemma app_substs_nontvar :
+  forall TI s, (exists TC, convert_type TI TC) -> app_substs s TI = TI.
+Proof.
+  introv H.
+  induction s as [|hd tl].
+  - reflexivity.
+  - destruct TI.
+    * simpl. rewrite IHtl. destruct hd. apply subst_nontvar. assumption.
+    * simpl. rewrite IHtl. destruct hd. apply subst_nontvar. assumption.
+    * simpl. rewrite IHtl. destruct hd. apply subst_nontvar. assumption.
+    * simpl. rewrite IHtl. destruct hd. apply subst_nontvar. assumption.
+    * inverts H. inverts H0.
+Qed.
+
+(*s
+Lemma app_substs_form_num :
+  forall s, app_substs s inft_Num = inft_Num.
+Proof.
+  introv.
+  assert (H: exists t, convert_type inft_Num t).
+    { exists cont_Num. apply CT_Num. }
+  apply (app_substs_nontvar inft_Num s). assumption.
+Qed.
+
+Lemma app_substs_form_bool :
+  forall s, app_substs s inft_Bool = inft_Bool.
+Proof.
+  introv.
+  assert (H: exists t, convert_type inft_Bool t).
+    { exists cont_Bool. apply CT_Bool. }
+  apply (app_substs_nontvar inft_Bool s). assumption.
+Qed. *)
+
+Lemma app_substs_form_list :
+  forall s t, exists t', app_substs s (inft_List t) = inft_List t'.
+Proof.
+  introv.
+  induction s as [|hd tl].
+  - exists t. reflexivity.
+  - simpl. inverts IHtl. rewrite H.
+    destruct hd. apply (subst_form_list i i0 x).
+Qed.
+
 (* ################################################################# *)
 (* Main goals *)
-(*
-Theorem typeinference_soundness :
-  forall (t : t_expr) (T : type)
-    (e : ut_expr) (env : environment) (fv : nat) (S : type) (C : constraint),
-  erase t e ->
-  typecheck env t T ->
-  typeinf env 0 e (fv, S, C) ->
-  (exists s, unify ((S, T)::C) s).
-Proof.
-  intros t T e env fv S C He Htc Hti.
-  destruct t.
-  - inverts He. inverts Hti. inverts Htc.
-    exists (@nil (id * type) % type). simpl. apply U_Identical with (t:=TNum).
-    * apply U_Empty.
-    * reflexivity.
-    * reflexivity.
-  - inverts He. inverts Hti. inverts Htc.
-    exists (@nil (id * type) % type). simpl. apply U_Identical with (t:=TBool).
-    * apply U_Empty.
-    * reflexivity.
-    * reflexivity.
-  - inverts He. inverts Hti. inverts Htc.
-    rewrite H1 in H3. inverts H3.
-    exists (@nil (id * type) % type). simpl. apply U_Identical with (t:=S).
-    * apply U_Empty.
-    * reflexivity.
-    * reflexivity.
-  - admit.
-  - admit.
-  - admit.
-  - admit.
-(*
-| U_ListList:
-    forall t1 t2 tl tl_sub
-      l1 l2 list_sub,
-    unify tl tl_sub ->
-    app_substs tl_sub t1 = TList l1 ->
-    app_substs tl_sub t2 = TList l2 ->
-    unify [(l1, l2)] list_sub ->
-    unify ((t1, t2)::tl) (list_sub ++ tl_sub)
-*)
-(*
-unify ((TList hd_T, TList T0) :: tl_C ++ hd_C ++ [(tl_T, TList hd_T)]) ?s
-*)
-  - inverts He. inverts Hti. inverts Htc. sort.
-    eexists.
-    apply U_ListList with
-  - inverts He. inverts Hti. inverts Htc.
-    exists [(Id 0, t)].
-    apply U_ListList with
-      (tl_sub:=[])
-      (list_sub:=[(Id 0, t)])
-      (l1:=TVar (Id 0))
-      (l2:=t).
-    * apply U_Empty.
-    * reflexivity.
-    * reflexivity.
-    * apply U_VarLeft.
-      + apply U_Empty.
-      + reflexivity.
-      + reflexivity.
-      + apply (occurs_nontvar (Id 0) t). assumption.
-Admitted.
-*)
-Theorem typeinference_soundness :
-  forall (t : t_expr) (T : type)
-    (e : ut_expr) (env : environment) (fv : nat) (S : type) (C : constraint),
-  erase t e ->
-  typecheck env t T ->
-  typeinf env 0 e (fv, S, C) ->
-  (exists (s : substitution), solution s C /\ app_substs s S = T).
-Proof.
-  introv He Htc Hti.
-  destruct t.
-  - inverts He. inverts Hti. inverts Htc.
-    exists (@nil (id * type) % type). simpl. split.
-    * apply SOL_Empty.
-    * reflexivity.
-  - inverts He. inverts Hti. inverts Htc.
-    exists (@nil (id * type) % type). simpl. split.
-    * apply SOL_Empty.
-    * reflexivity.
-  - inverts He. inverts Hti. inverts Htc.
-    rewrite H0 in H3. inverts H3.
-    exists (@nil (id * type) % type). simpl. split.
-    * apply SOL_Empty.
-    * reflexivity.
-  - admit.
-  - admit.
-  - admit.
-  - admit.
-  - admit.
-  - inverts He. inverts Hti. inverts Htc.
-    exists [(Id 0, t)]. split.
-    * apply SOL_Empty.
-    * reflexivity.
-Admitted.
 
+Theorem typeinference_soundness :
+  forall
+    t T tc_env
+    e S ti_env
+    C fv,
+  convert_expr t e ->
+  typecheck tc_env t T ->
+  typeinf ti_env 0 e (fv, S, C) ->
+  (forall i TC TI, tc_env i = Some TC /\ ti_env i = Some TI -> (exists s', convert_type (app_substs s' TI) TC)) ->
+  (exists s, solution s C /\ convert_type (app_substs s S) T).
+Proof.
+  introv Hc Htc Hti Hvar.
+  destruct t.
+  - inverts Hc. inverts Hti. inverts Htc.
+    exists (@nil (id * inft_type) % type). simpl. split.
+    * apply SOL_Empty.
+    * apply CT_Num.
+  - inverts Hc. inverts Hti. inverts Htc.
+    exists (@nil (id * inft_type) % type). simpl. split.
+    * apply SOL_Empty.
+    * apply CT_Bool.
+  - inverts Hc. inverts Hti. inverts Htc.
+    assert (Hconv: exists s', convert_type (app_substs s' S) T).
+        { apply (Hvar i T S). split. assumption. assumption. }
+    destruct Hconv.
+    exists x. split.
+    * apply SOL_Empty.
+    * assumption.
+  - admit.
+  - admit.
+  - admit.
+  - admit.
+  - admit.
+  - inverts Hc. inverts Hti. inverts Htc.
+    assert (HS': exists S', convert_type S' c).
+      { apply exists_inf_type_to_cont_type. }
+    destruct HS'.
+    exists [(Id 0, x)]. simpl. split.
+    * apply SOL_Empty.
+    * apply CT_List. assumption.
+Admitted.
 Theorem typeinference_completeness :
-  forall (e : ut_expr) (T : type) (env : environment) (fv : nat) (S : type) (C :constraint),
-  typeinf env 0 e (fv, S, C) ->
-  (exists (s : substitution),
-    solution s C /\
-    app_substs s S = T /\
-    vartype T = false) ->
-  (exists (t : t_expr), erase t e /\ typecheck env t T).
+  forall
+    (ti_env : ti_env) e fv S C T,
+  typeinf ti_env 0 e (fv, S, C) ->
+  (exists s, solution s C /\ convert_type (app_substs s S) T) ->
+  (exists t tc_env, convert_expr t e /\ typecheck tc_env t T).
 Proof.
   introv Hti Hsub.
-  destruct Hsub as [sub [Hsol [Happsub Hvartype]]]. sort.
+  destruct Hsub as [sub [Hsubsol Hsubconv]]. sort.
   induction e.
-  - exists (t_Num n). split.
-    * apply E_Num.
-    * inverts Hti. assert (Htnum: vartype TNum = false). { reflexivity. }
-      apply (app_substs_nontvar sub) in Htnum. rewrite Htnum in Happsub.
-      rewrite <- Happsub. apply TC_Num.
-  - exists (t_Bool b). split.
-    * apply E_Bool.
-    * inverts Hti. assert (Htbool: vartype TBool = false). { reflexivity. }
-      apply (app_substs_nontvar sub) in Htbool. rewrite Htbool in Happsub.
-      rewrite <- Happsub. apply TC_Bool.
+  - exists (t_Num n) (@empty cont_type). split.
+    * apply CE_Num.
+    * inverts Hti.
+      assert (Htnum: exists tc, convert_type inft_Num tc).
+        { exists cont_Num. apply CT_Num. }
+      apply (app_substs_nontvar inft_Num sub) in Htnum.
+      rewrite Htnum in Hsubconv. inverts Hsubconv. apply TC_Num.
+  - exists (t_Bool b) (@empty cont_type). split.
+    * apply CE_Bool.
+    * inverts Hti.
+      assert (Htbool: exists tc, convert_type inft_Bool tc).
+        { exists cont_Bool. apply CT_Bool. }
+      apply (app_substs_nontvar inft_Bool sub) in Htbool.
+      rewrite Htbool in Hsubconv. inverts Hsubconv. apply TC_Bool.
+  - exists (t_Var i) (update (@empty cont_type) i T). split.
+    * apply CE_Var.
+    * apply TC_Var. apply update_eq.
   - admit.
   - admit.
   - admit.
   - admit.
   - admit.
-  - admit.
-  - admit.
+  - inverts Hti.
+    assert (Hflist: exists t', app_substs sub (inft_List (inft_Var (Id 0))) = inft_List t').
+      { apply (app_substs_form_list sub (inft_Var (Id 0))). }
+    inverts Hflist. rewrite H in Hsubconv.
+    inverts Hsubconv.
+    exists (t_Nil l_t) (@empty cont_type). split.
+    * apply CE_Nil.
+    * apply TC_Nil.
 Admitted.
